src/QueryStructure/Automation/QSImplementation.v
@@ -1,0 +1,135 @@
+(* Tactics for extracting Query Structure Implementations. *)
+Require Export
+ADTSynthesis.Common.i2list2
+ADTSynthesis.QueryStructure.Implementation.DataStructures.Bags.BagsOfTuples
+ADTSynthesis.QueryStructure.Specification.Representation.QueryStructureNotations
+ADTSynthesis.QueryStructure.Automation.AutoDB.
+
+Ltac list_of_evar B As k :=
+  match As with
+    | nil => k (@nil B)
+    | cons ?a ?As' =>
+      makeEvar B ltac:(fun b =>
+                         list_of_evar
+                           B As' ltac:(fun Bs => k (cons b Bs)))
+  end.
+
+Definition LookupQSDelegateReps
+           {schemas : list NamedSchema}
+           (Reps : ilist (fun ns => Type) schemas)
+           (idx : @BoundedString (map relName schemas))
+: Type := ith_Bounded relName Reps idx.
+
+Definition LookupQSDelegateImpls
+           {schemas : list NamedSchema}
+           (SearchTerms : ilist (fun ns => SearchUpdateTerms (schemaHeading (relSchema ns))) schemas)
+           (Reps : ilist (fun ns => Type) schemas)
+           (DelegateImpls :
+              i2list2 (fun ns (SearchTerm : SearchUpdateTerms (schemaHeading (relSchema ns)))
+                           (Rep : Type)=>
+                         ComputationalADT.pcADT
+                           (BagSig (@Tuple (schemaHeading (relSchema ns)))
+                                   (BagSearchTermType SearchTerm)
+                                   (BagUpdateTermType SearchTerm))
+                           Rep) SearchTerms Reps)
+: forall (idx : @BoundedString (map relName schemas)),
+    ComputationalADT.pcADT
+      (Build_IndexedQueryStructure_Impl_Sigs SearchTerms idx)
+      (LookupQSDelegateReps Reps idx) := i2th2_Bounded relName DelegateImpls.
+
+Ltac BuildQSDelegateSigs QSImpl :=
+      let p := eval unfold QSImpl in QSImpl in
+          let p := eval simpl in (Sharpened_DelegateSigs p) in
+              match p with
+                  Build_IndexedQueryStructure_Impl_Sigs ?SearchTerms =>
+                  pose SearchTerms
+              end;
+        repeat match goal with
+                 | H : ilist _ (?sch :: ?schemas')
+                   |- ilist _ (?sch :: ?schemas') =>
+                   let SearchTerm := fresh "SearchTerm" in
+                   econstructor 1;
+                     [let SearchTerm := eval simpl in (ilist_hd H) in
+                          exact SearchTerm |
+                      let SearchTerm := eval simpl in (ilist_tl H) in
+                          pose SearchTerm; clear H ]
+                 | |- _ => econstructor 2
+               end.
+
+
+Ltac BuildQSDelegateReps QSImpl :=
+  let p := eval unfold QSImpl in QSImpl in
+      let p := eval simpl in (Sharpened_DelegateSigs p) in
+          match p with
+              Build_IndexedQueryStructure_Impl_Sigs ?SearchTerms =>
+              pose SearchTerms
+          end;
+          repeat match goal with
+                   | H : ilist _ (?sch :: ?schemas')
+                     |- ilist _ (?sch :: ?schemas') =>
+               let SearchTerm := fresh "SearchTerm" in
+               econstructor 1;
+                 [let SearchTerm := eval simpl in (BagSearchTermType (ilist_hd H)) in
+                      match SearchTerm
+                      with
+                        | BuildIndexSearchTerm ?AttrList =>
+                           pose AttrList;
+                             clear H;
+                             list_of_evar (@ProperAttribute (schemaHeading (relSchema sch))) AttrList
+                             ltac:(fun PAttrList =>
+                                     assert (map BagsOfTuples.Attribute PAttrList = AttrList)
+                                     by (simpl; repeat f_equal;
+                                         match goal with
+                                             |- @BagsOfTuples.Attribute ?heading ?h = ?g =>
+                                             instantiate (1 := @Build_ProperAttribute heading g _);
+                                             first [instantiate (1 := inright (eq_refl _))
+                                                   | instantiate (1 := inleft (inright (eq_refl _)))
+                                                   | instantiate (1 := inleft (inleft (right (eq_refl _))))
+                                                   | instantiate (1 := inleft (inleft (left (eq_refl _))))
+                                                   ]; reflexivity
+                                         end);
+                                   let p := eval simpl in (@NestedTreeFromAttributes _ PAttrList)
+                               in exact p)
+
+                                    (* Other SearchTerm types go here. *)
+                      end
+                 | let SearchTerm := eval simpl in (ilist_tl H) in
+                       pose SearchTerm; clear H ]
+             | |- _ => econstructor 2
+           end.
+
+Ltac BuildQSDelegateImpls QSImpl :=
+      repeat match goal with
+        | |- @i2list2 _ _ _ _
+                      (?sch :: ?schemas)
+                      (icons ?ST ?STs)
+                      (icons ?Rep ?Reps) =>
+          econstructor 1; simpl
+        | |- _ => econstructor 2
+      end;
+        match goal with
+            |- ComputationalADT.pcADT
+                 (BagSig (@Tuple ?heading)
+                         (BuildIndexSearchTerm ?AttrList) _) _ =>
+            list_of_evar (@ProperAttribute heading) AttrList
+                         ltac:(fun PAttrList =>
+                                 let H := fresh in
+                               try assert (map BagsOfTuples.Attribute PAttrList = AttrList) as H
+                               by (simpl; repeat f_equal;
+                                   match goal with
+                                       |- @BagsOfTuples.Attribute ?heading ?h = ?g =>
+                                       instantiate (1 := @Build_ProperAttribute heading g _);
+                                       first [instantiate (1 := inright (eq_refl _))
+                                             | instantiate (1 := inleft (inright (eq_refl _)))
+                                             | instantiate (1 := inleft (inleft (right (eq_refl _))))
+                                             | instantiate (1 := inleft (inleft (left (eq_refl _))))
+                                             ]; reflexivity
+                                   end);
+                             let p :=
+                                 eval simpl in (projT2 (@BagADTImpl _ _ _ _ (fun _ => true)
+                                                                     (@NestedTreeFromAttributesAsBag' _ PAttrList))) in clear H; exact p )
+      end.
+
+Arguments LookupQSDelegateReps _ _ _ / .
+Arguments LookupQSDelegateImpls _ _ _ _ _ / .
+Arguments Build_IndexedQueryStructure_Impl_cRep _ _ _ / .
