src/QueryStructure/Specification/Representation/QueryStructureNotations.v
@@ -1,8 +1,16 @@
 Require Export Coq.Strings.String Coq.omega.Omega Coq.Lists.List Coq.Logic.FunctionalExtensionality Coq.Sets.Ensembles
         ADTSynthesis.Common.Ensembles.IndexedEnsembles
-        ADTSynthesis.Computation ADTSynthesis.ADT ADTSynthesis.ADTRefinement ADTSynthesis.ADTNotation ADTSynthesis.QueryStructure.Specification.Representation.QueryStructureSchema
-        ADTSynthesis.ADTRefinement.BuildADTRefinements ADTSynthesis.QueryStructure.Specification.Operations.Query ADTSynthesis.QueryStructure.Specification.Operations.Insert ADTSynthesis.QueryStructure.Specification.Operations.Empty ADTSynthesis.QueryStructure.Specification.Operations.Update
-        ADTSynthesis.QueryStructure.Specification.Operations.Delete ADTSynthesis.QueryStructure.Specification.Representation.QueryStructure.
+        ADTSynthesis.Computation ADTSynthesis.ADT
+        ADTSynthesis.ADTRefinement ADTSynthesis.ADTNotation
+        ADTSynthesis.ADTRefinement.BuildADTRefinements
+        ADTSynthesis.QueryStructure.Specification.Representation.Notations
+        ADTSynthesis.QueryStructure.Specification.Representation.QueryStructureSchema
+        ADTSynthesis.QueryStructure.Specification.Representation.QueryStructure
+        ADTSynthesis.QueryStructure.Specification.Operations.Query
+        ADTSynthesis.QueryStructure.Specification.Operations.Insert
+        ADTSynthesis.QueryStructure.Specification.Operations.Empty
+        ADTSynthesis.QueryStructure.Specification.Operations.Update
+        ADTSynthesis.QueryStructure.Specification.Operations.Delete.
 
 Notation "heading / attr_index" := ((fun x : Attributes heading => x)
                                        {| bindex := attr_index; indexb := _ |})
